concurrency/verif_pair_conc.v
@@ -14,6 +14,8 @@ Definition t_struct_pair_impl := Tstruct _PairImpl noattr.
 Definition acquire_spec := DECLARE _acquire acquire_spec.
 Definition makelock_spec := DECLARE _makelock (makelock_spec _).
 Definition spawn_spec := DECLARE _spawn spawn_spec.
+Definition release_spec := DECLARE _release release_spec.
+Definition freelock_spec := DECLARE _freelock (freelock_spec _).
 Definition release2_spec := DECLARE _release2 release2_spec.
 Definition freelock2_spec := DECLARE _freelock2 (freelock2_spec _).
 
@@ -26,12 +28,13 @@ Notation pair_impl_info := (@G pair_impl_ghost).
 Definition pair_impl_state (p: val) (g: gname) (pair_impl: pair_impl_info): mpred :=
   EX content : Z, EX version: nat,
   !! (pair_impl = Some (content, version)) &&
-    (field_at Ews t_struct_pair_impl [StructField _data] (vint content) p *
-       field_at Ews t_struct_pair_impl [StructField _version] (vint version) p).
+    (field_at Ews t_struct_pair_impl (DOT _data) (vint content) p *
+       field_at Ews t_struct_pair_impl (DOT _version) (vint version) p).
 
 Definition pair_impl_rep (p: val) (g: gname) (sh: share) lock :=
-  field_at Ews t_struct_pair_impl [StructField _lock] lock p *
-    lock_inv sh lock (sync_inv g sh (pair_impl_state p)).
+  field_at sh t_struct_pair_impl (DOT _lock) lock p *
+    malloc_token sh tlock lock *
+    lock_inv sh lock (sync_inv g Tsh (pair_impl_state p)).
 
 Definition surely_malloc_spec :=
   DECLARE _surely_malloc
@@ -47,22 +50,30 @@ Definition surely_malloc_spec :=
        RETURN (p)
        SEP (mem_mgr gv; malloc_token Ews t p * data_at_ Ews t p).
 
-(* Definition pair_new_spec := *)
-(*   DECLARE _pair_new, *)
-(*     WITH gv: globals, *)
-(*       PRE [], *)
-(*       PROP (), *)
-(*       PARAMS (), *)
-(*       GLOBALS (gv), *)
-(*       SEP (mem_mgr gv), *)
-(*       POST [tptr t_struct_pair_impl], *)
-(*       PROP (), *)
-(*       LOCAL (temp ret_temp v), *)
-(*       SEP (mem_mgr gv) *)
+Definition pair_rep (g: gname) (value: Z) (version: nat) :=
+  public_half g (Some (value, version)).
+
+Definition pair_new_spec :=
+  DECLARE _pair_new
+    WITH gv: globals, value: Z
+    PRE [tint]
+      PROP ()
+      PARAMS (vint value)
+      GLOBALS (gv)
+      SEP (mem_mgr gv)
+    POST [tptr t_struct_pair_impl]
+      EX p: val, EX lock:val,  EX g: gname,
+      PROP ()
+      LOCAL (temp ret_temp p)
+      SEP (mem_mgr gv; pair_impl_rep p g Ews lock;
+           malloc_token Ews t_struct_pair_impl p;
+           pair_rep g value O).
 
 Definition Gprog : funspecs :=
-  ltac:(with_library prog [acquire_spec; release2_spec; makelock_spec;
-                           freelock2_spec; spawn_spec; surely_malloc_spec]).
+  ltac:(with_library prog [acquire_spec; release_spec; release2_spec; makelock_spec;
+                           freelock_spec; freelock2_spec; spawn_spec;
+                           surely_malloc_spec;
+                           pair_new_spec]).
 
 Lemma body_surely_malloc: semax_body Vprog Gprog f_surely_malloc surely_malloc_spec.
 Proof.
@@ -74,4 +85,25 @@ Proof.
   - forward_call 1. contradiction.
   - forward. rewrite -> if_false by auto; entailer!.
   - forward. rewrite -> if_false by auto. Exists p; entailer!.
+Qed.
+
+Lemma body_pair_new: semax_body Vprog Gprog f_pair_new pair_new_spec.
+Proof.
+  start_function.
+  forward_call (t_struct_pair_impl, gv).
+  Intros p.
+  forward_call (tlock, gv). { vm_compute; split; intro; easy. }
+  Intros lock.
+  ghost_alloc (both_halves (Some (value, O))). { apply @part_ref_valid. }
+  Intros g. rewrite <- both_halves_join. Intros.
+  forward_call (lock, Ews, (sync_inv g Tsh (pair_impl_state p))).
+  forward.
+  forward.
+  forward.
+  forward_call (lock, Ews, (sync_inv g Tsh (pair_impl_state p))). {
+    lock_props. unfold sync_inv, pair_impl_state.
+    Exists (Some (value, O)) value O. entailer !.
+    unfold_data_at (data_at Ews _ _ _). cancel. }
+  forward.
+  Exists p lock g. entailer !. unfold pair_impl_rep. cancel.
 Qed.
